Let smallstep get instruction from current state

SmallStep.v
@@ -65,8 +65,7 @@ Inductive step_res :=
 | sr_success: Ir.event -> Ir.Config.t -> step_res
 | sr_goes_wrong: step_res (* went wrong. *)
 | sr_oom: step_res (* out-of-memory *)
-| sr_nondet: step_res (* has non-deterministic result. *)
-| sr_prog_finish: Ir.val -> step_res (* program has finished (with following integer). *)
+| sr_prog_finish: Ir.val -> step_res (* program has finished (with a return value). *)
 .
 
 (****************************************************
@@ -198,195 +197,187 @@ Definition binop (bopc:Ir.Inst.bopcode) (i1 i2:N) (bsz:nat):N :=
   end.
 
 (* Semantics of an instruction which behaves deterministically.
+   If IR module of c is well-typed, and this function returns Some (result),
+   there is no possible execution other than the result.
    If running the instruction raises nondeterministic result,
-   this function returns sr_goes_wrong. *)
-Definition inst_det_step (c:Ir.Config.t) (i:Ir.Inst.t): step_res :=
-  match i with
-  | ibinop r (Ir.ity bsz) bopc op1 op2 =>
-    match (Ir.Config.get_val c op1, Ir.Config.get_val c op2) with
-    | (Some (Ir.num i1), Some (Ir.num i2)) =>
-      sr_success Ir.e_none (update_reg_and_incrpc c r (Ir.num (binop bopc i1 i2 bsz)))
-    | (Some Ir.poison, Some (Ir.num i2)) =>
-      sr_success Ir.e_none (update_reg_and_incrpc c r Ir.poison)
-    | (Some (Ir.num i2), Some Ir.poison) =>
-      sr_success Ir.e_none (update_reg_and_incrpc c r Ir.poison)
-    | (_, _) => sr_goes_wrong
-    end
-
-  | ipsub r (Ir.ity bsz) (Ir.ptrty opty) op1 op2 =>
-    match (Ir.Config.get_val c op1, Ir.Config.get_val c op2) with
-    | (Some (Ir.ptr p1), Some (Ir.ptr p2)) =>
-      sr_success Ir.e_none (update_reg_and_incrpc c r (psub p1 p2 (Ir.Config.m c) bsz))
-    | (Some Ir.poison, Some (Ir.ptr p2)) =>
-      sr_success Ir.e_none (update_reg_and_incrpc c r Ir.poison)
-    | (Some (Ir.ptr p1), Some Ir.poison) =>
-      sr_success Ir.e_none (update_reg_and_incrpc c r Ir.poison)
-    | (_, _) => sr_goes_wrong
-    end
-
-  | igep r (Ir.ptrty retty) opptr opidx inb =>
-    match (Ir.Config.get_val c opptr, Ir.Config.get_val c opidx) with
-    | (Some (Ir.ptr p), Some (Ir.num idx)) =>
-      sr_success Ir.e_none (update_reg_and_incrpc c r (gep p idx retty (Ir.Config.m c) inb))
-    | (Some Ir.poison, Some (Ir.num idx)) =>
-      sr_success Ir.e_none (update_reg_and_incrpc c r Ir.poison)
-    | (Some (Ir.ptr p), Some Ir.poison) =>
-      sr_success Ir.e_none (update_reg_and_incrpc c r Ir.poison)
-    | (_, _) => sr_goes_wrong
-    end
-
-  | iload r retty opptr =>
-    match (Ir.Config.get_val c opptr) with
-    | (Some (Ir.ptr p)) =>
-      if Ir.deref (Ir.Config.m c) p (Ir.ty_bytesz retty) then
-        sr_success Ir.e_none (update_reg_and_incrpc c r
-              (Ir.load_val (Ir.Config.m c) p retty))
-      else sr_goes_wrong
-    | _ => sr_goes_wrong
-    end
-
-  | istore valty opptr opval =>
-    match (Ir.Config.get_val c opptr, Ir.Config.get_val c opval) with
-    | (Some (Ir.ptr p), Some v) =>
-      if Ir.deref (Ir.Config.m c) p (Ir.ty_bytesz valty) then
-        sr_success Ir.e_none
-              (incrpc (Ir.Config.update_m c (Ir.store_val (Ir.Config.m c) p v valty)))
-      else sr_goes_wrong
-    | (_, _) => sr_goes_wrong
-    end
-
-  | imalloc r opty opval =>
-    (* malloc is not determinstic! *)
-    sr_nondet
-
-  | ifree opptr =>
-    match (Ir.Config.get_val c opptr) with
-    | Some (Ir.ptr p) =>
-      match (free p (Ir.Config.m c)) with
-      | Some m => sr_success Ir.e_none (incrpc (Ir.Config.update_m c m))
-      | None => sr_goes_wrong
+   this function returns None. *)
+Definition inst_det_step (c:Ir.Config.t): option step_res :=
+  match (Ir.Config.cur_inst c) with
+  | Some i =>
+    match i with
+    | ibinop r (Ir.ity bsz) bopc op1 op2 =>
+      match (Ir.Config.get_val c op1, Ir.Config.get_val c op2) with
+      | (Some (Ir.num i1), Some (Ir.num i2)) =>
+        Some (sr_success Ir.e_none (update_reg_and_incrpc c r (Ir.num (binop bopc i1 i2 bsz))))
+      | (Some Ir.poison, Some (Ir.num i2)) =>
+        Some (sr_success Ir.e_none (update_reg_and_incrpc c r Ir.poison))
+      | (Some (Ir.num i2), Some Ir.poison) =>
+        Some (sr_success Ir.e_none (update_reg_and_incrpc c r Ir.poison))
+      | (_, _) => Some sr_goes_wrong
       end
-    | _ => sr_goes_wrong
-    end
 
-  | ibitcast r opval retty =>
-    match (Ir.Config.get_val c opval) with
-    | Some (Ir.ptr p) =>
-      match retty with
-      | Ir.ptrty _ => sr_success Ir.e_none (update_reg_and_incrpc c r (Ir.ptr p))
-      | _ => sr_goes_wrong
+    | ipsub r (Ir.ity bsz) (Ir.ptrty opty) op1 op2 =>
+      match (Ir.Config.get_val c op1, Ir.Config.get_val c op2) with
+      | (Some (Ir.ptr p1), Some (Ir.ptr p2)) =>
+        Some (sr_success Ir.e_none (update_reg_and_incrpc c r (psub p1 p2 (Ir.Config.m c) bsz)))
+      | (Some Ir.poison, Some (Ir.ptr p2)) =>
+        Some (sr_success Ir.e_none (update_reg_and_incrpc c r Ir.poison))
+      | (Some (Ir.ptr p1), Some Ir.poison) =>
+        Some (sr_success Ir.e_none (update_reg_and_incrpc c r Ir.poison))
+      | (_, _) => Some sr_goes_wrong
       end
-    | Some (Ir.num n) =>
-      match retty with
-      | Ir.ity _ => sr_success Ir.e_none (update_reg_and_incrpc c r (Ir.num n))
-      | _ => sr_goes_wrong
+
+    | igep r (Ir.ptrty retty) opptr opidx inb =>
+      match (Ir.Config.get_val c opptr, Ir.Config.get_val c opidx) with
+      | (Some (Ir.ptr p), Some (Ir.num idx)) =>
+        Some (sr_success Ir.e_none (update_reg_and_incrpc c r (gep p idx retty (Ir.Config.m c) inb)))
+      | (Some Ir.poison, Some (Ir.num idx)) =>
+        Some (sr_success Ir.e_none (update_reg_and_incrpc c r Ir.poison))
+      | (Some (Ir.ptr p), Some Ir.poison) =>
+        Some (sr_success Ir.e_none (update_reg_and_incrpc c r Ir.poison))
+      | (_, _) => Some sr_goes_wrong
       end
-    | _ => sr_goes_wrong
-    end
 
-  | iptrtoint r opptr (Ir.ity retty) =>
-    match (Ir.Config.get_val c opptr) with
-    | Some (Ir.ptr p) =>
-      sr_success Ir.e_none
-                 (update_reg_and_incrpc c r (Ir.num (p2N p (Ir.Config.m c) retty)))
-    | Some (Ir.poison) =>
-      sr_success Ir.e_none (update_reg_and_incrpc c r Ir.poison)
-    | _ => sr_goes_wrong
-    end
-
-  | iinttoptr r opint (Ir.ptrty retty) =>
-    match (Ir.Config.get_val c opint) with
-    | Some (Ir.num n) =>
-      sr_success Ir.e_none (update_reg_and_incrpc c r
-        (Ir.ptr (Ir.pphy (N.to_nat n, nil, None))))
-    | Some (Ir.poison) =>
-      sr_success Ir.e_none (update_reg_and_incrpc c r Ir.poison)
-    | _=> sr_goes_wrong
-    end
-
-  | ievent opval =>
-    match (Ir.Config.get_val c opval) with
-    | Some (Ir.num n) => sr_success (Ir.e_some n) (incrpc c)
-    | _ => sr_goes_wrong
-    end
-
-  | iicmp_eq r opty op1 op2 =>
-    match (Ir.Config.get_val c op1, Ir.Config.get_val c op2) with
-    (* Integer comparison *)
-    | (Some (Ir.num n1), Some (Ir.num n2)) =>
-      sr_success Ir.e_none (update_reg_and_incrpc c r (to_num (N.eqb n1 n2)))
-    (* Comparison with poison *)
-    | (Some (Ir.poison), _) =>
-      sr_success Ir.e_none (update_reg_and_incrpc c r Ir.poison)
-    | (_, Some (Ir.poison)) =>
-      sr_success Ir.e_none (update_reg_and_incrpc c r Ir.poison)
-    (* Pointer comparison *)
-    | (Some (Ir.ptr p1), Some (Ir.ptr p2)) =>
-      match (icmp_eq_ptr p1 p2 (Ir.Config.m c)) with
-      | Some b =>  sr_success Ir.e_none (update_reg_and_incrpc c r (to_num b))
-      | None => sr_goes_wrong
+    | iload r retty opptr =>
+      match (Ir.Config.get_val c opptr) with
+      | (Some (Ir.ptr p)) =>
+        if Ir.deref (Ir.Config.m c) p (Ir.ty_bytesz retty) then
+          Some (sr_success Ir.e_none (update_reg_and_incrpc c r (Ir.load_val (Ir.Config.m c) p retty)))
+        else Some sr_goes_wrong
+      | _ => Some sr_goes_wrong
       end
-    | (_, _) => sr_goes_wrong (* In other cases, it is untyped. *)
-    end
 
-  | iicmp_ule r opty opptr1 opptr2 =>
-    match (Ir.Config.get_val c opptr1, Ir.Config.get_val c opptr2) with
-    (* Integer comparison *)
-    | (Some (Ir.num n1), Some (Ir.num n2)) =>
-      sr_success Ir.e_none (update_reg_and_incrpc c r (to_num (N.leb n1 n2)))
-    (* Comparison with poison *)
-    | (Some Ir.poison, _) =>
-      sr_success Ir.e_none (update_reg_and_incrpc c r Ir.poison)
-    | (_, Some Ir.poison) =>
-      sr_success Ir.e_none (update_reg_and_incrpc c r Ir.poison)
-    (* Comparison with pointer *)
-    | (Some (Ir.ptr p1), Some (Ir.ptr p2)) =>
-      match (icmp_ule_ptr p1 p2 (Ir.Config.m c)) with
-      | Some b => sr_success Ir.e_none (update_reg_and_incrpc c r (to_num b))
-      | None => sr_goes_wrong
+    | istore valty opptr opval =>
+      match (Ir.Config.get_val c opptr, Ir.Config.get_val c opval) with
+      | (Some (Ir.ptr p), Some v) =>
+        if Ir.deref (Ir.Config.m c) p (Ir.ty_bytesz valty) then
+          Some (sr_success Ir.e_none
+                           (incrpc (Ir.Config.update_m c (Ir.store_val (Ir.Config.m c) p v valty))))
+        else Some sr_goes_wrong
+      | (_, _) => Some sr_goes_wrong
       end
-    | (_, _) => sr_goes_wrong
+
+    | imalloc r opty opval =>
+      (* malloc is not determinstic! *)
+      None
+
+    | ifree opptr =>
+      match (Ir.Config.get_val c opptr) with
+      | Some (Ir.ptr p) =>
+        match (free p (Ir.Config.m c)) with
+        | Some m => Some (sr_success Ir.e_none (incrpc (Ir.Config.update_m c m)))
+        | None => Some sr_goes_wrong
+        end
+      | _ => Some sr_goes_wrong
+      end
+
+    | ibitcast r opval retty =>
+      match (Ir.Config.get_val c opval) with
+      | Some (Ir.ptr p) =>
+        match retty with
+        | Ir.ptrty _ => Some (sr_success Ir.e_none (update_reg_and_incrpc c r (Ir.ptr p)))
+        | _ => Some sr_goes_wrong
+        end
+      | Some (Ir.num n) =>
+        match retty with
+        | Ir.ity _ => Some (sr_success Ir.e_none (update_reg_and_incrpc c r (Ir.num n)))
+        | _ => Some sr_goes_wrong
+        end
+      | _ => Some sr_goes_wrong
+      end
+
+    | iptrtoint r opptr (Ir.ity retty) =>
+      match (Ir.Config.get_val c opptr) with
+      | Some (Ir.ptr p) =>
+        Some (sr_success Ir.e_none
+                         (update_reg_and_incrpc c r (Ir.num (p2N p (Ir.Config.m c) retty))))
+      | Some (Ir.poison) =>
+        Some (sr_success Ir.e_none (update_reg_and_incrpc c r Ir.poison))
+      | _ => Some sr_goes_wrong
+      end
+
+    | iinttoptr r opint (Ir.ptrty retty) =>
+      match (Ir.Config.get_val c opint) with
+      | Some (Ir.num n) =>
+        Some (sr_success Ir.e_none (update_reg_and_incrpc c r
+                                                          (Ir.ptr (Ir.pphy (N.to_nat n, nil, None)))))
+      | Some (Ir.poison) =>
+        Some (sr_success Ir.e_none (update_reg_and_incrpc c r Ir.poison))
+    | _=> Some sr_goes_wrong
     end
 
-  | _ => sr_goes_wrong (* Untyped IR *)
+    | ievent opval =>
+      match (Ir.Config.get_val c opval) with
+      | Some (Ir.num n) => Some (sr_success (Ir.e_some n) (incrpc c))
+      | _ => Some sr_goes_wrong
+      end
+
+    | iicmp_eq r opty op1 op2 =>
+      match (Ir.Config.get_val c op1, Ir.Config.get_val c op2) with
+      (* Integer comparison *)
+      | (Some (Ir.num n1), Some (Ir.num n2)) =>
+        Some (sr_success Ir.e_none (update_reg_and_incrpc c r (to_num (N.eqb n1 n2))))
+      (* Comparison with poison *)
+      | (Some (Ir.poison), _) =>
+        Some (sr_success Ir.e_none (update_reg_and_incrpc c r Ir.poison))
+      | (_, Some (Ir.poison)) =>
+        Some (sr_success Ir.e_none (update_reg_and_incrpc c r Ir.poison))
+      (* Pointer comparison *)
+      | (Some (Ir.ptr p1), Some (Ir.ptr p2)) =>
+        match (icmp_eq_ptr p1 p2 (Ir.Config.m c)) with
+        | Some b => Some (sr_success Ir.e_none (update_reg_and_incrpc c r (to_num b)))
+        | None => None (* nondet. result *)
+        end
+      | (_, _) => Some sr_goes_wrong (* In other cases, it is untyped. *)
+      end
+
+    | iicmp_ule r opty opptr1 opptr2 =>
+      match (Ir.Config.get_val c opptr1, Ir.Config.get_val c opptr2) with
+      (* Integer comparison *)
+      | (Some (Ir.num n1), Some (Ir.num n2)) =>
+        Some (sr_success Ir.e_none (update_reg_and_incrpc c r (to_num (N.leb n1 n2))))
+      (* Comparison with poison *)
+      | (Some Ir.poison, _) =>
+        Some (sr_success Ir.e_none (update_reg_and_incrpc c r Ir.poison))
+      | (_, Some Ir.poison) =>
+        Some (sr_success Ir.e_none (update_reg_and_incrpc c r Ir.poison))
+      (* Comparison with pointer *)
+      | (Some (Ir.ptr p1), Some (Ir.ptr p2)) =>
+        match (icmp_ule_ptr p1 p2 (Ir.Config.m c)) with
+        | Some b => Some (sr_success Ir.e_none (update_reg_and_incrpc c r (to_num b)))
+        | None => None
+        end
+      | (_, _) => Some sr_goes_wrong
+      end
+
+    | _ => Some sr_goes_wrong (* Untyped IR *)
+    end
+
+  | None => Some sr_goes_wrong
   end.
 
 (* Inductive definition of small-step semantics of instruction.
    Note that sr_nondet is never used in inst_step. *)
-Inductive inst_step: Ir.Config.t -> Ir.Inst.t -> step_res -> Prop :=
-| s_binop: forall c i r retty bopc op1 op2
-      (HINST:i = Ir.Inst.ibinop r retty bopc op1 op2),
-    inst_step c i (inst_det_step c i)
-
-| s_psub: forall c i r retty ptrty opptr1 opptr2
-      (HINST:i = Ir.Inst.ipsub r retty ptrty opptr1 opptr2),
-    inst_step c i (inst_det_step c i)
-
-| s_gep: forall c i r retty opptr opidx inb
-      (HINST:i = Ir.Inst.igep r retty opptr opidx inb),
-    inst_step c i (inst_det_step c i)
-
-| s_load: forall c i r retty opptr
-      (HINST:i = Ir.Inst.iload r retty opptr),
-    inst_step c i (inst_det_step c i)
-
-| s_store: forall c i valty opval opptr
-      (HINST:i = Ir.Inst.istore valty opval opptr),
-    inst_step c i (inst_det_step c i)
+Inductive inst_step: Ir.Config.t -> step_res -> Prop :=
+| s_det: forall c sr
+      (HNEXT:Some sr = inst_det_step c), inst_step c sr
 
 | s_malloc_zero: forall c i r szty opsz
+      (HCUR:Some i = Ir.Config.cur_inst c)
       (HINST:i = Ir.Inst.imalloc r szty opsz)
       (HZERO:Ir.Config.get_val c opsz = Some (Ir.num 0%N)),
-    inst_step c i (sr_success Ir.e_none (update_reg_and_incrpc c r (Ir.ptr Ir.NULL)))
+    inst_step c (sr_success Ir.e_none (update_reg_and_incrpc c r (Ir.ptr Ir.NULL)))
 
 | s_malloc_oom: forall c i r szty opsz nsz
+      (HCUR:Some i = Ir.Config.cur_inst c)
       (HINST:i = Ir.Inst.imalloc r szty opsz)
       (HSZ:Some (Ir.num nsz) = Ir.Config.get_val c opsz)
       (HNOSPACE:~exists (P:list nat),
             Ir.Memory.allocatable (Ir.Config.m c) (List.map (fun addr => (addr, N.to_nat nsz)) P) = true),
-    inst_step c i sr_oom
+    inst_step c sr_oom
 
 | s_malloc: forall c i r szty opsz nsz (P:list nat) m' l contents
+      (HCUR:Some i = Ir.Config.cur_inst c)
       (HINST:i = Ir.Inst.imalloc r szty opsz)
       (HSZ:Some (Ir.num nsz) = Ir.Config.get_val c opsz)
       (HSZ2:N.to_nat nsz > 0)
@@ -398,31 +389,12 @@ Inductive inst_step: Ir.Config.t -> Ir.Inst.t -> step_res -> Prop :=
                        (List.map (fun addr => (addr, N.to_nat nsz)) P) = true)
       (HNEW: (m', l) = Ir.Memory.new (Ir.Config.m c) (Ir.heap) (N.to_nat nsz)
                                      (Ir.SYSALIGN) contents P HMBWF HDISJ),
-    inst_step c i (sr_success Ir.e_none (update_reg_and_incrpc
+    inst_step c (sr_success Ir.e_none (update_reg_and_incrpc
                                            (Ir.Config.update_m c m') r
                     (Ir.ptr (Ir.plog (l, 0)))))
 
-| s_free: forall c i opptr
-      (HINST:i = Ir.Inst.ifree opptr),
-    inst_step c i (inst_det_step c i)
-
-| s_bitcast: forall c i r opval retty
-      (HINST:i = Ir.Inst.ibitcast r opval retty),
-    inst_step c i (inst_det_step c i)
-
-| s_ptrtoint: forall c i r opptr retty
-      (HINST:i = Ir.Inst.iptrtoint r opptr retty),
-    inst_step c i (inst_det_step c i)
-
-| s_inttoptr: forall c i r opint retty
-      (HINST:i = Ir.Inst.iinttoptr r opint retty),
-    inst_step c i (inst_det_step c i)
-
-| s_event: forall c i opval
-      (HINST:i = Ir.Inst.ievent opval),
-    inst_step c i (inst_det_step c i)
-
 | s_icmp_eq_nondet: forall c i r opty op1 op2 mb1 mb2 l1 o1 l2 o2 res
+      (HCUR:Some i = Ir.Config.cur_inst c)
       (HINST:i = Ir.Inst.iicmp_eq r opty op1 op2)
       (HOP1:Some (Ir.ptr (Ir.plog (l1, o1))) = Ir.Config.get_val c op1)
       (HOP2:Some (Ir.ptr (Ir.plog (l2, o2))) = Ir.Config.get_val c op2)
@@ -431,14 +403,10 @@ Inductive inst_step: Ir.Config.t -> Ir.Inst.t -> step_res -> Prop :=
       (HDIFF:~l1 = l2)
       (HNOTINB:~(o1 < Ir.MemBlock.n mb1 /\ o2 < Ir.MemBlock.n mb2))
       (HNONDET:res = 0%N \/ res = 1%N),
-    inst_step c i (sr_success Ir.e_none (update_reg_and_incrpc c r (Ir.num res)))
-
-| s_icmp_eq: forall c i r opty op1 op2 c'
-      (HINST:i = Ir.Inst.iicmp_eq r opty op1 op2)
-      (HC':sr_success Ir.e_none c' = inst_det_step c i),
-    inst_step c i (sr_success Ir.e_none c')
+    inst_step c (sr_success Ir.e_none (update_reg_and_incrpc c r (Ir.num res)))
 
 | s_icmp_ule_nondet_diff: forall c i r opty op1 op2 mb1 mb2 l1 l2 o1 o2 res
+      (HCUR:Some i = Ir.Config.cur_inst c)
       (HINST:i = Ir.Inst.iicmp_ule r opty op1 op2)
       (HOP1:Some (Ir.ptr (Ir.plog (l1, o1))) = Ir.Config.get_val c op1)
       (HOP2:Some (Ir.ptr (Ir.plog (l2, o2))) = Ir.Config.get_val c op2)
@@ -446,21 +414,17 @@ Inductive inst_step: Ir.Config.t -> Ir.Inst.t -> step_res -> Prop :=
       (HMB2:Some mb2 = Ir.Memory.get (Ir.Config.m c) l2)
       (HDIFF:~l1 = l2)
       (HNONDET:res = 0%N \/ res = 1%N),
-    inst_step c i (sr_success Ir.e_none (update_reg_and_incrpc c r (Ir.num res)))
+    inst_step c (sr_success Ir.e_none (update_reg_and_incrpc c r (Ir.num res)))
 
 | s_icmp_ule_nondet_same: forall c i r opty op1 op2 mb l o1 o2 res
+      (HCUR:Some i = Ir.Config.cur_inst c)
       (HINST:i = Ir.Inst.iicmp_ule r opty op1 op2)
       (HOP1:Some (Ir.ptr (Ir.plog (l, o1))) = Ir.Config.get_val c op1)
       (HOP2:Some (Ir.ptr (Ir.plog (l, o2))) = Ir.Config.get_val c op2)
       (HMB:Some mb = Ir.Memory.get (Ir.Config.m c) l)
       (HNOTINB:~(o1 <= Ir.MemBlock.n mb /\ o2 <= Ir.MemBlock.n mb))
       (HNONDET:res = 0%N \/ res = 1%N),
-    inst_step c i (sr_success Ir.e_none (update_reg_and_incrpc c r (Ir.num res)))
-
-| s_icmp_ule: forall c i r opty op1 op2 c'
-      (HINST:i = Ir.Inst.iicmp_ule r opty op1 op2)
-      (HC':sr_success Ir.e_none c' = inst_det_step c i),
-    inst_step c i (sr_success Ir.e_none c')
+    inst_step c (sr_success Ir.e_none (update_reg_and_incrpc c r (Ir.num res)))
 .
 
 (* Categorization of instructions. *)
@@ -692,50 +656,145 @@ Ltac des_op c op op' HINV :=
 Ltac des_inv v HINV :=
   destruct (v); try (inversion HINV; fail).
 
+(* Lemma: inst_det_step preserves well-formedness of configuration. *)
+Lemma inst_det_step_wf:
+  forall c c' i e
+         (HWF:Ir.Config.wf c)
+         (HCUR:Some i = Ir.Config.cur_inst c)
+         (HNEXT:Some (sr_success e c') = inst_det_step c),
+    Ir.Config.wf c'.
+Proof.
+    intros.
+    unfold inst_det_step in HNEXT. (* ibinop. *)
+    rewrite <- HCUR in HNEXT.
+    destruct i as [r retty bopc op1 op2 (* ibinop *)
+                  |r retty ptrty opptr1 opptr2 (* ipsub *)
+                  |r retty opptr opidx inb (* igep *)
+                  |r retty opptr (* iload *)
+                  |valty opval opptr (* istore *)
+                  |(* imalloc *)
+                  |opptr (* ifree *)
+                  |r opval retty (* ibitcast *)
+                  |r opptr retty (* iptrtoint *)
+                  |r opint retty (* iinttoptr *)
+                  |opval (* ievent *)
+                  |r opty op1 op2 (* iicmp_eq *)
+                  |r opty op1 op2 (* iicmp_ule *)
+                  ] eqn:HINST; try (inversion HNEXT; fail).
+    + rename HNEXT into H2.
+      destruct bopc.
+      { simpl in H2.
+        des_inv retty H2. des_op c op1 opv1 H2. des_op c op2 opv2 H2.
+        + des_inv opv1 H2; des_inv opv2 H2; inversion H2; thats_it.
+        + des_inv opv1 H2.
+      }
+      { simpl in H2.
+        des_inv retty H2. des_op c op1 opv1 H2. des_op c op2 opv2 H2.
+        + des_inv opv1 H2; des_inv opv2 H2; inversion H2; thats_it.
+        + des_inv opv1 H2.
+      }
+    + (* ipsub. *)
+      rename HNEXT into H2. simpl in H2.
+      des_inv retty H2. des_inv ptrty H2. des_op c opptr1 op1 H2.
+      des_inv op1 H2; des_op c opptr2 op2 H2; des_inv op2 H2; inversion H2; thats_it.
+    + (* igep. *)
+      rename HNEXT into H2. simpl in H2.
+      des_inv retty H2. des_op c opptr op1 H2.
+      des_inv op1 H2; des_op c opidx op2 H2; des_inv op2 H2; inversion H2; thats_it.
+    + (* iload. *)
+      rename HNEXT into H2. simpl in H2. des_op c opptr op1 H2.
+      des_inv op1 H2. des_ifH H2; try (inversion H2; fail). inversion H2. thats_it.
+    + (* istore. *)
+      rename HNEXT into H2. simpl in H2.
+      des_op c opval opv H2. des_inv opv H2. des_op c opptr opp H2.
+      destruct (Ir.deref (Ir.Config.m c) p (Ir.ty_bytesz valty)) eqn:Hderef;
+        try (inversion H2; fail).
+      inversion H2.
+      apply incrpc_wf with (c := Ir.Config.update_m c (Ir.store_val (Ir.Config.m c) p opp valty));
+        try reflexivity.
+      destruct HWF.
+      split; simpl; try assumption.
+      eapply Ir.store_val_wf. eassumption. reflexivity.  congruence.
+    + (* ifree *)
+      destruct HWF. rename HNEXT into H2. simpl in H2.
+      des_op c opptr opp H2. des_inv opp H2.
+      destruct (free p (Ir.Config.m c)) as [m0 | ] eqn:Hfree; try (inversion H2; fail).
+      inversion H2.
+      unfold free in Hfree.
+      destruct p.
+      { destruct p. destruct n; try (inversion Hfree).
+        apply incrpc_wf with (c := Ir.Config.update_m c m0).
+        assert (HWF':Ir.Memory.wf m0).
+        { eapply Ir.Memory.free_wf. eapply wf_m. erewrite Hfree. reflexivity. }
+        split; try (simpl; assumption). reflexivity. }
+      { destruct p. destruct p.
+        destruct (Ir.Memory.zeroofs_block (Ir.Config.m c) n) eqn:Hblk.
+        -- destruct p.
+           des_ifH Hfree.
+           apply incrpc_wf with (c := Ir.Config.update_m c m0).
+           assert (HWF':Ir.Memory.wf m0).
+           { eapply Ir.Memory.free_wf. eapply wf_m. erewrite Hfree. reflexivity. }
+           split; try (simpl; assumption). reflexivity.
+           inversion Hfree.
+        -- inversion Hfree. }
+    + (* ibitcast. *)
+      rename HNEXT into H2. simpl in H2.
+      des_op c opval opv H2. des_inv opv H2; des_inv retty H2; inversion H2; thats_it.
+    + (* iptrtoint. *)
+      rename HNEXT into H2. simpl in H2. des_inv retty H2.
+      des_op c opptr opp H2. des_inv opp H2; inversion H2; thats_it.
+    + (* iinttoptr *)
+      rename HNEXT into H2. simpl in H2. des_inv retty H2.
+      des_op c opint opi H2. des_inv opi H2; inversion H2; thats_it.
+    + (* ievent *)
+      rename HNEXT into H2. simpl in H2.
+      des_op c opval opv H2. des_inv opv H2.
+      inversion H2. eapply incrpc_wf. eassumption. reflexivity.
+    + (* iicmp_eq, det *)
+      rename HNEXT into HC'. simpl in HC'.
+      des_op c op1 op1v HC'.
+      { destruct op1v.
+        - des_op c op2 op2v HC'.
+          destruct op2v; inversion HC'; thats_it.
+        - des_op c op2 op2v HC'.
+          destruct op2v; try (inversion HC'; fail).
+          destruct (icmp_eq_ptr p p0 (Ir.Config.m c)) eqn:Heq_ptr; try (inversion HC'; fail);
+             inversion HC'; thats_it.
+          inversion HC'. thats_it.
+        - inversion HC'. thats_it. }
+      { des_op c op2 op2v HC'.
+        destruct op2v; try (inversion HC'; fail).
+        inversion HC'. thats_it. }
+    + (* iicmp_ule, det *)
+      rename HNEXT into HC'. simpl in HC'.
+      des_op c op1 op1v HC'.
+      { des_inv op1v HC';
+          des_op c op2 op2v HC'.
+        -- des_inv op2v HC'; inversion HC'; thats_it.
+        -- des_inv op2v HC'.
+           { destruct (icmp_ule_ptr p p0 (Ir.Config.m c)) eqn:Huleptr; try (inversion HC'; fail).
+             inversion HC'. thats_it. }
+           { inversion HC'. thats_it. }
+        -- inversion HC'. thats_it.
+        -- inversion HC'. thats_it. }
+      { des_op c op2 op2v HC'. des_inv op2v HC'. inversion HC'. thats_it. }
+Qed.
+
 (* Theorem: inst_step preserves well-formedness of configuration. *)
 Theorem inst_step_wf:
-  forall c i c' e
+  forall c c' e
          (HWF:Ir.Config.wf c)
-         (HSTEP:inst_step c i (sr_success e c')),
+         (HSTEP:inst_step c (sr_success e c')),
     Ir.Config.wf c'.
 Proof.
   intros.
   inversion HSTEP.
-  - (* ibinop. *)
-    rewrite HINST in H2.
-    destruct bopc.
-    { simpl in H2.
-      des_inv retty H2. des_op c op1 opv1 H2. des_op c op2 opv2 H2.
-      + des_inv opv1 H2; des_inv opv2 H2; inversion H2; thats_it.
-      + des_inv opv1 H2.
-    }
-    { simpl in H2.
-      des_inv retty H2. des_op c op1 opv1 H2. des_op c op2 opv2 H2.
-      + des_inv opv1 H2; des_inv opv2 H2; inversion H2; thats_it.
-      + des_inv opv1 H2.
-    }
-  - (* ipsub. *)
-    rewrite HINST in H2. simpl in H2.
-    des_inv retty H2. des_inv ptrty H2. des_op c opptr1 op1 H2.
-    des_inv op1 H2; des_op c opptr2 op2 H2; des_inv op2 H2; inversion H2; thats_it.
-  - (* igep. *)
-    rewrite HINST in H2. simpl in H2.
-    des_inv retty H2. des_op c opptr op1 H2.
-    des_inv op1 H2; des_op c opidx op2 H2; des_inv op2 H2; inversion H2; thats_it.
-  - (* iload. *)
-    rewrite HINST in H2. simpl in H2. des_op c opptr op1 H2.
-    des_inv op1 H2. des_ifH H2; try (inversion H2; fail). inversion H2. thats_it.
-  - (* istore. *)
-    rewrite HINST in H2. simpl in H2.
-    des_op c opval opv H2. des_inv opv H2. des_op c opptr opp H2.
-    destruct (Ir.deref (Ir.Config.m c) p (Ir.ty_bytesz valty)) eqn:Hderef;
-      try (inversion H2; fail).
-    inversion H2.
-    apply incrpc_wf with (c := Ir.Config.update_m c (Ir.store_val (Ir.Config.m c) p opp valty));
-      try reflexivity.
-    destruct HWF.
-    split; simpl; try assumption.
-    eapply Ir.store_val_wf. eassumption. reflexivity.  congruence.
+  - unfold inst_det_step in HNEXT.
+    destruct (Ir.Config.cur_inst c) as [i0|] eqn:Hcur.
+    eapply inst_det_step_wf. eassumption.
+    rewrite Hcur. reflexivity. unfold inst_det_step.
+    rewrite Hcur. eassumption.
+    inversion HNEXT.
   - (* imalloc with size 0 *)
     thats_it.
   - (* imalloc, succeed *)
@@ -746,77 +805,14 @@ Proof.
         eapply wf_m.
         eapply HNEW.
     + reflexivity.
-  - (* ifree *)
-    destruct HWF. rewrite HINST in H2. simpl in H2.
-    des_op c opptr opp H2. des_inv opp H2.
-    destruct (free p (Ir.Config.m c)) as [m0 | ] eqn:Hfree; try (inversion H2; fail).
-    inversion H2.
-    unfold free in Hfree.
-    destruct p.
-    + destruct p. destruct n; try (inversion Hfree).
-      apply incrpc_wf with (c := Ir.Config.update_m c m0).
-      assert (HWF':Ir.Memory.wf m0).
-      { eapply Ir.Memory.free_wf. eapply wf_m. erewrite Hfree. reflexivity. }
-      split; try (simpl; assumption). reflexivity.
-    + destruct p. destruct p.
-      destruct (Ir.Memory.zeroofs_block (Ir.Config.m c) n) eqn:Hblk.
-      * destruct p.
-        des_ifH Hfree.
-        apply incrpc_wf with (c := Ir.Config.update_m c m0).
-        assert (HWF':Ir.Memory.wf m0).
-        { eapply Ir.Memory.free_wf. eapply wf_m. erewrite Hfree. reflexivity. }
-        split; try (simpl; assumption). reflexivity.
-        inversion Hfree.
-      * inversion Hfree.
-  - (* ibitcast. *)
-    rewrite HINST in H2. simpl in H2.
-    des_op c opval opv H2. des_inv opv H2; des_inv retty H2; inversion H2; thats_it.
-  - (* iptrtoint. *)
-    rewrite HINST in H2. simpl in H2. des_inv retty H2.
-    des_op c opptr opp H2. des_inv opp H2; inversion H2; thats_it.
-  - (* iinttoptr *)
-    rewrite HINST in H2. simpl in H2. des_inv retty H2.
-    des_op c opint opi H2. des_inv opi H2; inversion H2; thats_it.
-  - (* ievent *)
-    rewrite HINST in H2. simpl in H2.
-    des_op c opval opv H2. des_inv opv H2.
-    inversion H2. eapply incrpc_wf. eassumption. reflexivity.
   - (* iicmp_eq, nondet *)
     eapply update_reg_and_incrpc_wf.
     eassumption.
     reflexivity.
-  - (* iicmp_eq, det *)
-    rewrite HINST in HC'. simpl in HC'.
-    des_op c op1 op1v HC'.
-    + destruct op1v.
-      * des_op c op2 op2v HC'.
-        destruct op2v; inversion HC'; thats_it.
-      * des_op c op2 op2v HC'.
-        destruct op2v; try (inversion HC'; fail).
-        destruct (icmp_eq_ptr p p0 (Ir.Config.m c)) eqn:Heq_ptr; try (inversion HC'; fail);
-        inversion HC'; thats_it.
-        inversion HC'. thats_it.
-      * inversion HC'. thats_it.
-    + des_op c op2 op2v HC'.
-      destruct op2v; try (inversion HC'; fail).
-      inversion HC'. thats_it.
   - (* icmp_ule, nondet *)
     eapply update_reg_and_incrpc_wf. eassumption. reflexivity.
   - (* icmp_ule, nondet 2 *)
     eapply update_reg_and_incrpc_wf. eassumption. reflexivity.
-  - (* icmp_ule, det *)
-    rewrite HINST in HC'. simpl in HC'.
-    des_op c op1 op1v HC'.
-    + des_inv op1v HC';
-      des_op c op2 op2v HC'.
-      * des_inv op2v HC'; inversion HC'; thats_it.
-      * des_inv op2v HC'.
-        -- destruct (icmp_ule_ptr p p0 (Ir.Config.m c)) eqn:Huleptr; try (inversion HC'; fail).
-           inversion HC'. thats_it.
-        -- inversion HC'. thats_it.
-      * inversion HC'. thats_it.
-      * inversion HC'. thats_it.
-    + des_op c op2 op2v HC'. des_inv op2v HC'. inversion HC'. thats_it.
 Qed.
 
 (****************************************************
@@ -847,83 +843,123 @@ Proof.
   des_ifs.
 Qed.
 
+(* Lemma: inst_det_step preserves well-formedness of configuration. *)
+Ltac thats_it2 := apply no_mem_change_after_update.
+
+Lemma changes_mem_spec_det:
+  forall c c' i e
+         (HWF:Ir.Config.wf c)
+         (HCUR:Some i = Ir.Config.cur_inst c)
+         (HNOMEMCHG:changes_mem i = false)
+         (HNEXT:Some (sr_success e c') = inst_det_step c),
+    c.(Ir.Config.m) = c'.(Ir.Config.m).
+Proof.
+    intros.
+    unfold inst_det_step in HNEXT. (* ibinop. *)
+    rewrite <- HCUR in HNEXT.
+    destruct i as [r retty bopc op1 op2 (* ibinop *)
+                  |r retty ptrty opptr1 opptr2 (* ipsub *)
+                  |r retty opptr opidx inb (* igep *)
+                  |r retty opptr (* iload *)
+                  |valty opval opptr (* istore *)
+                  |(* imalloc *)
+                  |opptr (* ifree *)
+                  |r opval retty (* ibitcast *)
+                  |r opptr retty (* iptrtoint *)
+                  |r opint retty (* iinttoptr *)
+                  |opval (* ievent *)
+                  |r opty op1 op2 (* iicmp_eq *)
+                  |r opty op1 op2 (* iicmp_ule *)
+                  ] eqn:HINST; try (inversion HNEXT; fail);
+      try (inversion HNOMEMCHG; fail).
+    + rename HNEXT into H2.
+      destruct bopc.
+      { simpl in H2.
+        des_inv retty H2. des_op c op1 opv1 H2. des_op c op2 opv2 H2.
+        + des_inv opv1 H2; des_inv opv2 H2; inversion H2; thats_it2.
+        + des_inv opv1 H2.
+      }
+      { simpl in H2.
+        des_inv retty H2. des_op c op1 opv1 H2. des_op c op2 opv2 H2.
+        + des_inv opv1 H2; des_inv opv2 H2; inversion H2; thats_it2.
+        + des_inv opv1 H2.
+      }
+    + (* ipsub. *)
+      rename HNEXT into H2. simpl in H2.
+      des_inv retty H2. des_inv ptrty H2. des_op c opptr1 op1 H2.
+      des_inv op1 H2; des_op c opptr2 op2 H2; des_inv op2 H2; inversion H2; thats_it2.
+    + (* igep. *)
+      rename HNEXT into H2. simpl in H2.
+      des_inv retty H2. des_op c opptr op1 H2.
+      des_inv op1 H2; des_op c opidx op2 H2; des_inv op2 H2; inversion H2; thats_it2.
+    + (* iload. *)
+      rename HNEXT into H2. simpl in H2. des_op c opptr op1 H2.
+      des_inv op1 H2. des_ifH H2; try (inversion H2; fail). inversion H2. thats_it2.
+    + (* ibitcast. *)
+      rename HNEXT into H2. simpl in H2.
+      des_op c opval opv H2. des_inv opv H2; des_inv retty H2; inversion H2; thats_it2.
+    + (* iptrtoint. *)
+      rename HNEXT into H2. simpl in H2. des_inv retty H2.
+      des_op c opptr opp H2. des_inv opp H2; inversion H2; thats_it2.
+    + (* iinttoptr *)
+      rename HNEXT into H2. simpl in H2. des_inv retty H2.
+      des_op c opint opi H2. des_inv opi H2; inversion H2; thats_it2.
+    + (* ievent *)
+      rename HNEXT into H2. simpl in H2.
+      des_op c opval opv H2. des_inv opv H2.
+      inversion H2. eapply no_mem_change_after_incrpc.
+    + (* iicmp_eq, det *)
+      rename HNEXT into HC'. simpl in HC'.
+      des_op c op1 op1v HC'.
+      { destruct op1v.
+        - des_op c op2 op2v HC'.
+          destruct op2v; inversion HC'; thats_it2.
+        - des_op c op2 op2v HC'.
+          destruct op2v; try (inversion HC'; fail).
+          destruct (icmp_eq_ptr p p0 (Ir.Config.m c)) eqn:Heq_ptr; try (inversion HC'; fail);
+             inversion HC'; thats_it2.
+          inversion HC'. thats_it2.
+        - inversion HC'. thats_it2. }
+      { des_op c op2 op2v HC'.
+        destruct op2v; try (inversion HC'; fail).
+        inversion HC'. thats_it2. }
+    + (* iicmp_ule, det *)
+      rename HNEXT into HC'. simpl in HC'.
+      des_op c op1 op1v HC'.
+      { des_inv op1v HC';
+          des_op c op2 op2v HC'.
+        -- des_inv op2v HC'; inversion HC'; thats_it2.
+        -- des_inv op2v HC'.
+           { destruct (icmp_ule_ptr p p0 (Ir.Config.m c)) eqn:Huleptr; try (inversion HC'; fail).
+             inversion HC'. thats_it2. }
+           { inversion HC'. thats_it2. }
+        -- inversion HC'. thats_it2.
+        -- inversion HC'. thats_it2. }
+      { des_op c op2 op2v HC'. des_inv op2v HC'. inversion HC'. thats_it2. }
+Qed.
+
 (* Theorem: if changes_mem returns false, memory isn't
    changed after inst_step. *)
 Theorem changes_mem_spec:
   forall c i c' e
          (HWF:Ir.Config.wf c)
+         (HCUR:Some i = Ir.Config.cur_inst c)
          (HNOMEMCHG:changes_mem i = false)
-         (HSTEP:inst_step c i (sr_success e c')),
+         (HSTEP:inst_step c (sr_success e c')),
     c.(Ir.Config.m) = c'.(Ir.Config.m).
 Proof.
   intros.
-  inversion HSTEP; try (rewrite HINST in HNOMEMCHG; inversion HNOMEMCHG; fail).
-  - (* ibinop. *)
-    rewrite HINST in H2.
-    destruct bopc.
-    { simpl in H2.
-      des_inv retty H2. des_op c op1 opv1 H2. des_op c op2 opv2 H2.
-      + des_inv opv1 H2; des_inv opv2 H2; inversion H2; apply no_mem_change_after_update.
-      + des_inv opv1 H2.
-    }
-    { simpl in H2.
-      des_inv retty H2. des_op c op1 opv1 H2. des_op c op2 opv2 H2.
-      + des_inv opv1 H2; des_inv opv2 H2; inversion H2; apply no_mem_change_after_update.
-      + des_inv opv1 H2.
-    }
-  - (* ipsub. *)
-    rewrite HINST in H2. simpl in H2.
-    des_inv retty H2. des_inv ptrty H2. des_op c opptr1 op1 H2.
-    des_inv op1 H2; des_op c opptr2 op2 H2; des_inv op2 H2; inversion H2; apply no_mem_change_after_update.
-  - (* igep. *)
-    rewrite HINST in H2. simpl in H2.
-    des_inv retty H2. des_op c opptr op1 H2.
-    des_inv op1 H2; des_op c opidx op2 H2; des_inv op2 H2; inversion H2; apply no_mem_change_after_update.
-  - (* iload. *)
-    rewrite HINST in H2. simpl in H2. des_op c opptr op1 H2.
-    des_inv op1 H2. des_ifH H2; try (inversion H2; fail). inversion H2. apply no_mem_change_after_update.
-  - (* ibitcast. *)
-    rewrite HINST in H2. simpl in H2.
-    des_op c opval opv H2. des_inv opv H2; des_inv retty H2; inversion H2; apply no_mem_change_after_update.
-  - (* iptrtoint. *)
-    rewrite HINST in H2. simpl in H2. des_inv retty H2.
-    des_op c opptr opp H2. des_inv opp H2; inversion H2; apply no_mem_change_after_update.
-  - (* iinttoptr *)
-    rewrite HINST in H2. simpl in H2. des_inv retty H2.
-    des_op c opint opi H2. des_inv opi H2; inversion H2; apply no_mem_change_after_update.
-  - (* ievent *)
-    rewrite HINST in H2. simpl in H2.
-    des_op c opval opv H2. des_inv opv H2.
-    inversion H2. apply no_mem_change_after_incrpc.
+  inversion HSTEP.
+  - eapply changes_mem_spec_det. assumption.
+    eassumption. assumption. eassumption.
+  - (* malloc, NULL *)
+    apply no_mem_change_after_update.
+  - (* malloc *)
+    rewrite <- HCUR in HCUR0. inversion HCUR0. rewrite H3 in HINST.
+    rewrite HINST in HNOMEMCHG. inversion HNOMEMCHG.
   - (* iicmp_eq, nondet *) apply no_mem_change_after_update.
-  - (* iicmp_eq, det *)
-    rewrite HINST in HC'. simpl in HC'.
-    des_op c op1 op1v HC'.
-    + destruct op1v.
-      * des_op c op2 op2v HC'.
-        destruct op2v; inversion HC'; apply no_mem_change_after_update.
-      * des_op c op2 op2v HC'. des_inv op2v HC'.
-        destruct (icmp_eq_ptr p p0 (Ir.Config.m c)) eqn:Heq_ptr; try (inversion HC'; fail);
-        inversion HC'; apply no_mem_change_after_update.
-        inversion HC'. apply no_mem_change_after_update.
-      * inversion HC'. apply no_mem_change_after_update.
-    + des_op c op2 op2v HC'. des_inv op2v HC'.
-      inversion HC'. apply no_mem_change_after_update.
   - (* icmp_ule, nondet *) apply no_mem_change_after_update.
   - (* icmp_ule, nondet 2 *) apply no_mem_change_after_update.
-  - (* icmp_ule, det *)
-    rewrite HINST in HC'. simpl in HC'.
-    des_op c op1 op1v HC'.
-    + des_inv op1v HC';
-      des_op c op2 op2v HC'.
-      * des_inv op2v HC'; inversion HC'; apply no_mem_change_after_update.
-      * des_inv op2v HC'.
-        -- destruct (icmp_ule_ptr p p0 (Ir.Config.m c)) eqn:Huleptr; try (inversion HC'; fail).
-           inversion HC'. apply no_mem_change_after_update.
-        -- inversion HC'. apply no_mem_change_after_update.
-      * inversion HC'. apply no_mem_change_after_update.
-      * inversion HC'. apply no_mem_change_after_update.
-    + des_op c op2 op2v HC'. des_inv op2v HC'. inversion HC'. apply no_mem_change_after_update.
 Qed.
 
 End SmallStep.
